LeanLgtm/Lang.lean
@@ -1,0 +1,749 @@
+import Ssreflect.Lang
+import Mathlib.Data.Finmap
+import LeanLgtm.Util
+
+
+open Classical
+
+/- =========================== Language Syntax =========================== -/
+
+inductive prim where
+  | val_ref : prim
+  | val_get : prim
+  | val_set : prim
+  | val_free : prim
+  | val_neg : prim
+  | val_opp : prim
+  | val_eq : prim
+  | val_add : prim
+  | val_neq : prim
+  | val_sub : prim
+  | val_mul : prim
+  | val_div : prim
+  | val_mod : prim
+  | val_rand : prim
+  | val_le : prim
+  | val_lt : prim
+  | val_ge : prim
+  | val_gt : prim
+  | val_ptr_add : prim
+
+abbrev loc := Nat
+abbrev var := String
+
+def null : loc := 0
+
+mutual
+  inductive val : Type where
+    | val_unit : val
+    | val_bool : Bool → val
+    | val_int : Int → val
+    | val_loc : loc → val
+    | val_prim : prim → val
+    | val_fun : var -> trm -> val
+    | val_fix : var -> var -> trm -> val
+    | val_uninit : val
+    | val_error : val
+
+  inductive trm : Type where
+    | trm_val : val -> trm
+    | trm_var : var -> trm
+    | trm_fun : var -> trm -> trm
+    | trm_fix : var -> var -> trm -> trm
+    | trm_app : trm -> trm -> trm
+    | trm_seq : trm -> trm -> trm
+    | trm_let : var -> trm -> trm -> trm
+    | trm_if : trm -> trm -> trm -> trm
+end
+
+/- States and heaps are represented as finite maps -/
+abbrev state := Finmap (λ _ : loc ↦ val)
+abbrev heap := state
+
+
+/- ============================= Notations ============================= -/
+
+/- val and term are inhabited -/
+instance : Inhabited val where
+  default := val.val_unit
+
+instance : Inhabited trm where
+  default := trm.trm_val (val.val_unit)
+
+/- Coercions -/
+instance : Coe Bool val where
+  coe b := val.val_bool b
+
+instance : Coe Int val where
+  coe z := val.val_int z
+
+/- Help Lean to treat Nat as val -/
+instance : OfNat val n where
+  ofNat := val.val_int n
+
+instance : Coe loc val where
+  coe l := val.val_loc l
+
+instance : Coe prim val where
+  coe x := val.val_prim x
+
+instance : Coe val trm where
+  coe v := trm.trm_val v
+
+instance : Coe var trm where
+  coe x := trm.trm_var x
+
+instance : CoeFun trm (fun _ => trm -> trm) where
+  coe x := trm.trm_app x
+
+/- ================== Terms, Values and Substitutions ================== -/
+open trm
+
+abbrev trm_is_val : trm → Prop
+  | trm_val _ => true
+  | _         => false
+
+/- Capture-avoiding substitution -/
+def subst (y : var) (v' : val) (t : trm) : trm :=
+  -- let aux x := subst y v' x
+  let if_y_eq x t1 t2 := if x = y then t1 else t2
+  match t with
+  | trm_val v => trm_val v
+  | trm_var x => if_y_eq x (trm_val v') t
+  | trm_fun x t1 => trm_fun x (if_y_eq x t1 (subst y v' t1))
+  | trm_fix f x t1 => trm_fix f x (if_y_eq f t1 (if_y_eq x t1 (subst y v' t1)))
+  | trm_app t1 t2 => trm_app (subst y v' t1) (subst y v' t2)
+  | trm_seq t1 t2 => trm_seq (subst y v' t1) (subst y v' t2)
+  | trm_let x t1 t2 => trm_let x (subst y v' t1) (if_y_eq x t2 (subst y v' t2))
+  | trm_if t0 t1 t2 => trm_if (subst y v' t0) (subst y v' t1) (subst y v' t2)
+
+noncomputable def is_true (P : Prop) : Bool :=
+  if P then true else false
+
+
+/- ======================= Small-Step Semantics ======================= -/
+open val
+open prim
+
+/- Function for reading a memory location (to unwrap the option) -/
+def read_state (p : loc) (h : state) :=
+  match Finmap.lookup p h with
+  | some v => v
+  | none   => default
+
+inductive step : state → trm → state → trm → Prop where
+
+  -- Context Rules
+  | step_seq_ctx : forall s1 s2 t1 t1' t2,
+      step s1 t1 s2 t1' →
+      step s1 (trm_seq t1 t2) s2 (trm_seq t1' t2)
+  | step_let_ctx : forall s1 s2 x t1 t1' t2,
+      step s1 t1 s2 t1' →
+      step s1 (trm_let x t1 t2) s2 (trm_let x t1' t2)
+  | step_app_arg_1 : forall s1 s2 t1 t1' t2,
+      step s1 t1 s2 t1' →
+      step s1 (trm_app t1 t2) s2 (trm_app t1' t2)
+  | step_app_arg2 : forall s1 s2 v1 t2 t2',
+      step s1 t2 s2 t2' →
+      step s1 (trm_app v1 t2) s2 (trm_app v1 t2')
+
+  -- Reduction
+  | step_fun : forall s x t1,
+      step s (trm_fun x t1) s (val_fun x t1)
+  | step_fix : forall s f x t1,
+      step s (trm_fix f x t1) s (val_fix f x t1)
+  | step_app_fun : forall s v1 v2 x t1,
+      v1 = val_fun x t1 →
+      v2 = trm_val v2' →
+      step s (trm_app v1 v2) s (subst x v2' t1)
+  | step_app_fix : forall s v1 v2 f x t1,
+      v1 = val_fix f x t1 →
+      v2 = trm_val v2' →
+      step s (trm_app v1 v2) s (subst x v2' (subst f v1 t1))
+  | step_if : forall s b t1 t2,
+      step s (trm_if (val_bool b) t1 t2) s (if b then t1 else t2)
+  | step_seq : forall s t2 v1,
+      step s (trm_seq v1 t2) s t2
+  | step_let : forall s x t2 v1,
+      v1 = trm_val v1' →
+      step s (trm_let x v1 t2) s (subst x v1' t2)
+
+  -- Unary Operations
+  | step_neg : forall s b,
+      step s (trm_app val_neg (val_bool b)) s (val_bool (¬ b))
+  | step_opp : forall s n,
+      step s (trm_app val_opp (val_int n)) s (val_int (- n))
+  | step_rand : forall s n n1,
+      0 <= n1 ∧ n1 < n →
+      step s (trm_app val_rand (val_int n)) s (val_int n1)
+
+  -- Binary Operations
+  | step_eq : forall s v1 v2,
+      step s (trm_app (trm_app val_eq v1) v2) s (val_bool (is_true (v1 = v2)))
+  | step_neq : forall s v1 v2,
+      step s (trm_app (trm_app val_neq v1) v2) s (val_bool (is_true (v1 ≠ v2)))
+  | step_add : forall s n1 n2,
+      step s (trm_app (trm_app val_add (val_int n1)) (val_int n2)) s
+        (val_int (n1 + n2))
+  | step_sub : forall s n1 n2,
+      step s (trm_app (trm_app val_sub (val_int n1)) (val_int n2)) s
+        (val_int (n1 - n2))
+  | step_mul : forall s n1 n2,
+      step s (trm_app (trm_app val_mul (val_int n1)) (val_int n2)) s
+        (val_int (n1 * n2))
+  | step_div : forall s n1 n2,
+      n2 ≠ 0 →
+      step s (trm_app (trm_app val_div (val_int n1)) (val_int n2)) s
+        (n1 / n2)
+  | step_mod : forall s n1 n2,
+      n2 ≠ 0 →
+      step s (trm_app (trm_app val_mod (val_int n1)) (val_int n2)) s
+        (n1 % n2)
+  | step_le : forall s n1 n2,
+      step s (trm_app (trm_app val_le (val_int n1)) (val_int n2)) s
+        (val_bool (n1 <= n2))
+  | step_lt : forall s n1 n2,
+      step s (trm_app (trm_app val_lt (val_int n1)) (val_int n2)) s
+        (val_bool (n1 < n2))
+  | step_ge : forall s n1 n2,
+      step s (trm_app (trm_app val_ge (val_int n1)) (val_int n2)) s
+        (val_bool (n1 >= n2))
+  | step_gt : forall s n1 n2,
+      step s (trm_app (trm_app val_gt (val_int n1)) (val_int n2)) s
+        (val_bool (n1 > n2))
+  | step_ptr_add : forall s p1 p2 n,
+      (p2:ℤ) = (p1:loc) + n →
+      step s (trm_app (trm_app val_ptr_add (val_loc p1)) (val_int n)) s
+        (val_loc (Int.toNat p2))
+
+  -- Heap Opeartions
+  | step_ref : forall s v p,
+      ¬ p ∈ s →
+      v = trm_val v' →
+      step s (trm_app val_ref v) (Finmap.insert p v' s) (val_loc p)
+  | step_get : forall s p,
+      p ∈ s →
+      step s (trm_app val_get (val_loc p)) s (read_state p s)
+  | step_set : forall s p v,
+      p ∈ s ->
+      v = trm_val v' →
+      step s (trm_app (trm_app val_set (val_loc p)) v)
+        (Finmap.insert p v' s) val_unit
+  | step_free : forall s p,
+      p ∈ s →
+      step s (trm_app val_free (val_loc p)) (Finmap.erase p s) val_unit
+
+/- Multi-step relation -/
+inductive steps : state → trm → state → trm → Prop :=
+  | steps_refl : forall s t,
+      steps s t s t
+  | steps_step : forall s1 s2 s3 t1 t2 t3,
+      step s1 t1 s2 t2 →
+      steps s2 t2 s3 t3 →
+      steps s1 t1 s3 t3
+
+lemma steps_of_step s1 s2 t1 t2 :
+  step s1 t1 s2 t2 → steps s1 t1 s2 t2 :=
+by
+  sby move=> ?; apply steps.steps_step
+
+lemma steps_trans s1 s2 s3 t1 t2 t3 :
+  steps s1 t1 s2 t2 →
+  steps s2 t2 s3 t3 →
+  steps s1 t1 s3 t3 := by sby elim
+
+/- Predicate [reducible s t] for asserting that [(s, t)] can step -/
+def reducible (s : state) (t : trm) : Prop :=
+  exists s' t', step s t s' t'
+
+/- The configuration [(s, t)] is not stuck, i.e. [notstuck s t] if either
+   t is a value or [(s, t)] can step -/
+def notstuck (s : state) (t : trm) : Prop :=
+  trm_is_val t \/ reducible s t
+
+
+/- ========== Big-step Semantics for Primitive Operations ========== -/
+
+/- Big-step relation for unary operators -/
+inductive evalunop : prim → val → (val → Prop) → Prop where
+  | evalunop_neg : forall b1,
+      evalunop val_neg (val_bool b1) (fun v => v = val_bool (¬ b1))
+  | evalunop_opp : forall n1,
+      evalunop val_opp (val_int n1) (fun v => v = val_int (- n1))
+  | evalunop_rand : forall n,
+      n > 0 →
+      evalunop val_rand (val_int n)
+        (fun r => exists n1, r = val_int n1 ∧ 0 <= n1 ∧ n1 < n)
+
+/- Big-step relation for binary operators -/
+inductive evalbinop : val → val → val → (val->Prop) → Prop where
+  | evalbinop_eq : forall v1 v2,
+      evalbinop val_eq v1 v2 (fun v => v = val_bool (is_true (v1 = v2)))
+  | evalbinop_neq : forall v1 v2,
+      evalbinop val_neq v1 v2 (fun v => v = val_bool (is_true (v1 ≠ v2)))
+  | evalbinop_add : forall n1 n2,
+      evalbinop val_add (val_int n1) (val_int n2)
+        (fun v => v = val_int (n1 + n2))
+  | evalbinop_sub : forall n1 n2,
+      evalbinop val_sub (val_int n1) (val_int n2)
+        (fun v => v = val_int (n1 - n2))
+  | evalbinop_mul : forall n1 n2,
+      evalbinop val_mul (val_int n1) (val_int n2)
+        (fun v => v = val_int (n1 * n2))
+  | evalbinop_div : forall n1 n2,
+      ¬(n2 = 0) →
+      evalbinop val_div (val_int n1) (val_int n2)
+        (fun v => v = val_int (n1 / n2))
+  | evalbinop_mod : forall n1 n2,
+      ¬(n2 = 0) →
+      evalbinop val_mod (val_int n1) (val_int n2)
+        (fun v => v = val_int (n1 % n2))
+  | evalbinop_le : forall n1 n2,
+      evalbinop val_le (val_int n1) (val_int n2)
+        (fun v => v = val_bool (n1 <= n2))
+  | evalbinop_lt : forall n1 n2,
+      evalbinop val_lt (val_int n1) (val_int n2)
+        (fun v => v = val_bool (n1 < n2))
+  | evalbinop_ge : forall n1 n2,
+      evalbinop val_ge (val_int n1) (val_int n2)
+        (fun v => v = val_bool (n1 >= n2))
+  | evalbinop_gt : forall n1 n2,
+      evalbinop val_gt (val_int n1) (val_int n2)
+        (fun v => v = val_bool (n1 > n2))
+
+  -- Not really sure what's going on in the last rule here since
+  -- in the original CFML code, p2 doesn't have to be a valid pointer (it has
+  -- type int and could be negative), so not sure if this is semantically
+  -- equivalent to what was here before.
+  | evalbinop_ptr_add : forall p1 p2 n,
+      (p2:ℤ) = (p1:loc) + n ->
+      evalbinop val_ptr_add (val_loc p1) (val_int n)
+        (fun v => v = val_loc (Int.toNat p2))
+
+
+/- ========================= Big-step Semantics ========================= -/
+
+section eval
+
+/- Predicate for converting predicates [P : val → Prop] into postconditions
+   of type [val → state → Prop] that hold in state s -/
+def purepost (s : state) (P : val → Prop) : val → state → Prop :=
+  fun v s' => P v ∧ s' = s
+
+def purepostin (s : state) (P : val → Prop) (Q : val → state → Prop) : Prop :=
+  -- Equivalent to [purepost S P ===> Q]
+  forall v, P v → Q v s
+
+variable (Q : val → state → Prop)
+
+/- Big-step relation -/
+inductive eval : state → trm → (val → state → Prop) -> Prop where
+  | eval_val : forall s v Q,
+      Q v s ->
+      eval s (trm_val v) Q
+  | eval_fun : forall s x t1 Q,
+      Q (val_fun x t1) s ->
+      eval s (trm_fun x t1) Q
+  | eval_fix : forall s f x t1 Q,
+      Q (val_fix f x t1) s ->
+      eval s (trm_fix f x t1) Q
+  | eval_app_arg1 : forall s1 t1 t2 Q1 Q,
+      ¬ trm_is_val t1 ->
+      eval s1 t1 Q1 ->
+      (forall v1 s2, Q1 v1 s2 -> eval s2 (trm_app v1 t2) Q) ->
+      eval s1 (trm_app t1 t2) Q
+  | eval_app_arg2 : forall s1 v1 t2 Q1 Q,
+      ¬ trm_is_val t2 ->
+      eval s1 t2 Q1 ->
+      (forall v2 s2, Q1 v2 s2 -> eval s2 (trm_app v1 v2) Q) ->
+      eval s1 (trm_app v1 t2) Q
+  | eval_app_fun : forall s1 v1 v2 x t1 Q,
+      v1 = val_fun x t1 ->
+      eval s1 (subst x v2 t1) Q ->
+      eval s1 (trm_app v1 v2) Q
+  | eval_app_fix : forall s v1 v2 f x t1 Q,
+      v1 = val_fix f x t1 ->
+      eval s (subst x v2 (subst f v1 t1)) Q ->
+      eval s (trm_app v1 v2) Q
+  | eval_seq : forall Q1 s t1 t2 Q,
+      eval s t1 Q1 ->
+      (forall v1 s2, Q1 v1 s2 -> eval s2 t2 Q) ->
+      eval s (trm_seq t1 t2) Q
+  | eval_let : forall Q1 s x t1 t2 Q,
+      eval s t1 Q1 ->
+      (forall v1 s2, Q1 v1 s2 -> eval s2 (subst x v1 t2) Q) ->
+      eval s (trm_let x t1 t2) Q
+  | eval_if : forall s (b : Bool) t1 t2 Q,
+      eval s (if b then t1 else t2) Q ->
+      eval s (trm_if (val_bool b) t1 t2) Q
+  | eval_unop : forall op s v1 P Q,
+      evalunop op v1 P ->
+      purepostin s P Q ->
+      eval s (trm_app op v1) Q
+  | eval_binop : forall op s v1 v2 P Q,
+      evalbinop op v1 v2 P ->
+      purepostin s P Q ->
+      eval s (trm_app (trm_app op v1) v2) Q
+  | eval_ref : forall s v Q,
+      v = trm_val v' ->
+      (forall p, ¬ p ∈ s ->
+          Q (val_loc p) (Finmap.insert p v' s)) ->
+      eval s (trm_app val_ref v) Q
+  | eval_get : forall s p Q,
+      p ∈ s ->
+      Q (read_state p s) s ->
+      eval s (trm_app val_get (val_loc p)) Q
+  | eval_set : forall s p v Q,
+      v = trm_val v' ->
+      p ∈ s ->
+      Q val_unit (Finmap.insert p v' s) ->
+      eval s (trm_app (trm_app val_set (val_loc p)) v) Q
+  | eval_free : forall s p Q,
+      p ∈ s ->
+      Q val_unit (Finmap.erase p s) ->
+      eval s (trm_app val_free (val_loc p)) Q
+
+/- Not sure if the rules eval_ref and eval_set are correct. I had to add the
+   condition [v = trm_val v'] to get the definition to type-check. However, this
+   assertion says that the term v is a value but really shouldn't this be
+   that v big-steps to a value? Not sure what the best way to do this is.
+   Perhaps by doing something like the seq rule where there is some
+   intermediate condition Q' for first evaluating v and then composing that
+   with the memory allocation. -/
+
+/- Rule for values to instantiate postconditions -/
+
+lemma eval_val_minimal s v :
+  eval s (trm_val v) (fun v' s' => (v' = v) /\ (s' = s)) :=
+  by sby apply eval.eval_val
+
+
+/- Special rules to avoid unecessary use of [evalbinop] and [evalunop] -/
+
+lemma eval_add  s n1 n2 Q :
+  Q (val_int (n1 + n2)) s →
+  eval s (trm_app (trm_app val_add (val_int n1)) (val_int n2)) Q :=
+by
+  move=> ?
+  apply eval.eval_binop
+  { apply evalbinop.evalbinop_add }
+  sdone
+
+lemma eval_div s n1 n2 Q :
+  n2 ≠ 0 ->
+  Q (val_int (n1 / n2)) s ->
+  eval s (trm_app (trm_app val_div (val_int n1)) (val_int n2)) Q :=
+by
+  move=> *
+  apply eval.eval_binop
+  { apply evalbinop.evalbinop_div=>// }
+  sdone
+
+lemma eval_rand s (n : ℤ) Q :
+  n > 0 ->
+  (forall n1, 0 <= n1 ∧ n1 < n -> Q n1 s) ->
+  eval s (trm_app val_rand (val_int n)) Q :=
+by
+  move=> *
+  apply eval.eval_unop
+  { apply evalunop.evalunop_rand=>// }
+  sby move=> ? []
+
+
+/- Derived rules for reasoning about applications that don't require checking
+   if terms are already values -/
+
+lemma eval_app_arg1' s1 t1 t2 Q1 Q :
+  eval s1 t1 Q1 ->
+  (forall v1 s2, Q1 v1 s2 -> eval s2 (trm_app v1 t2) Q) ->
+  eval s1 (trm_app t1 t2) Q :=
+by
+  move=> hevals1 hevals2
+  scase: [(trm_is_val t1)]=> hVal
+  { sby apply eval.eval_app_arg1 }
+  sby scase: t1=> // ? []
+
+/- TODO: optimise (similar to ↑) -/
+lemma eval_app_arg2' : forall s1 v1 t2 Q1 Q,
+  eval s1 t2 Q1 ->
+  (forall v2 s2, eval s2 (trm_app v1 v2) Q) ->
+  eval s1 (trm_app v1 t2) Q :=
+by
+  move=> s1 v1 t2 Q1 Q hevals1 hevals2
+  scase: [(trm_is_val t2)]=> hVal
+  { apply eval.eval_app_arg2=>// }
+  sby scase: t2
+
+
+/- [eval_like t1 t2] asserts that [t2] evaluates like [t1], i.e.,
+    this relation holds whenever [t2] reduces in small-step to [t1]. -/
+def eval_like (t1 t2:trm) : Prop :=
+  forall s Q, eval s t1 Q -> eval s t2 Q
+
+end eval
+
+/- ================================================================= -/
+/-* ** Notation for Concrete Terms -/
+
+declare_syntax_cat lang
+declare_syntax_cat args
+
+syntax ident : lang
+syntax num : lang
+syntax lang "(" lang,* ")" : lang
+syntax "if " lang "then " lang "end " : lang
+syntax ppIndent("if " lang " then") ppSpace lang ppDedent(ppSpace) ppRealFill("else " lang) : lang
+syntax "let" ident " := " lang " in" ppDedent(ppLine lang) : lang
+-- syntax withPosition("let" ident " := " lang) " in " lang : lang
+syntax lang ";\n" ppDedent(lang) : lang
+syntax "fun" ident+ " => " lang : lang
+syntax "fix" ident ident+ " => " lang : lang
+syntax "fun_ " ident* " => " lang : lang
+syntax "fix_ " ident ident* " => " lang : lang
+syntax "()" : lang
+syntax "ref" : lang
+syntax "free" : lang
+syntax "not" : lang
+syntax "!" noWs lang : lang
+syntax "-" noWs lang : lang
+syntax lang " := " lang : lang
+syntax lang " + " lang : lang
+syntax lang " * " lang : lang
+syntax lang " - " lang : lang
+syntax lang " / " lang : lang
+syntax lang " < " lang : lang
+syntax lang " > " lang : lang
+syntax lang " = " lang : lang
+syntax lang " <= " lang : lang
+syntax lang " >= " lang : lang
+syntax lang " != " lang : lang
+syntax lang " mod " lang : lang
+syntax "(" lang ")" : lang
+
+syntax "[lang|\n" lang "]" : term
+
+
+local notation "%" x => (Lean.quote (toString (Lean.Syntax.getId x)))
+
+def trm_apps (f:trm) (ts:List trm) : trm :=
+  match ts with
+  | [] => f
+  | ti::ts' => trm_apps (trm_app f ti) ts'
+
+def trm_funs (xs:List var) (t:trm) : trm :=
+  match xs with
+  | [] => t
+  | x1::xs' => trm_fun x1 (trm_funs xs' t)
+
+def val_funs (xs:List var) (t:trm) : val :=
+  match xs with
+  | [] => panic! "function with zero argumets!"
+  | x1::xs' => val_fun x1 (trm_funs xs' t)
+
+def trm_fixs (f:var) (xs:List var) (t:trm) : trm :=
+  match xs with
+  | [] => t
+  | x1::xs' => trm_fix f x1 (trm_funs xs' t)
+
+def val_fixs (f:var) (xs:List var) (t:trm) : val :=
+  match xs with
+  | .nil => val_uninit
+  | x1::xs' => val_fix f x1 (trm_funs xs' t)
+
+macro_rules
+  | `([lang| ()])                       => `(trm_val val_unit)
+  | `([lang| $n:num])                   => `(trm_val (val_int $n))
+  | `([lang| $x:ident])                 => `(trm_var $(%x))
+  | `([lang| $t1 ( $t2,* )])                  => do
+    `(trm_apps [lang| $t1] [ $[[lang|$t2]],* ])
+  | `([lang| if $t1 then $t2 else $t3]) => `(trm_if [lang| $t1] [lang| $t2] [lang| $t3])
+  | `([lang| if $t1 then $t2 end])      => `(trm_if [lang| $t1] [lang| $t2] (trm_val val_unit))
+  | `([lang| let $x := $t1:lang in $t2:lang])     =>
+    `(trm_let $(%x) [lang| $t1] [lang| $t2])
+  | `([lang| $t1 ; $t2])                => `(trm_seq [lang| $t1] [lang| $t2])
+  | `([lang| fun_ $xs* => $t])             => do
+    let xs <- xs.mapM fun x => `(term| $(%x))
+    `(trm_funs [ $xs,* ] [lang| $t])
+  | `([lang| fun $xs* => $t])             => do
+    let xs <- xs.mapM fun x => `(term| $(%x))
+    `(val_funs [ $xs,* ] [lang| $t])
+  | `([lang| fix_ $f $xs* => $t])    => do
+      let xs <- xs.mapM fun x => `(term| $(%x))
+      `(trm_fixs $(%f) [ $xs,* ] [lang| $t])
+  | `([lang| fix $f $xs* => $t])    => do
+      let xs <- xs.mapM fun x => `(term| $(%x))
+      `(val_fixs $(%f) [ $xs,* ] [lang| $t])
+  | `([lang| ref])                      => `(trm_val (val_prim val_ref))
+  | `([lang| free])                     => `(trm_val (val_prim val_free))
+  | `([lang| not])                      => `(trm_val (val_prim val_not))
+  | `([lang| !$t])                      => `(trm_val val_get [lang| $t])
+  | `([lang| $t1 := $t2])               => `(trm_val val_set [lang| $t1] [lang| $t2])
+  | `([lang| $t1 + $t2])                => `(trm_val val_add [lang| $t1] [lang| $t2])
+  | `([lang| $t1 * $t2])                => `(trm_val val_mul [lang| $t1] [lang| $t2])
+  | `([lang| $t1 - $t2])                => `(trm_val val_sub [lang| $t1] [lang| $t2])
+  | `([lang| $t1 / $t2])                => `(trm_val val_div [lang| $t1] [lang| $t2])
+  | `([lang| $t1 < $t2])                => `(trm_val val_lt [lang| $t1] [lang| $t2])
+  | `([lang| $t1 > $t2])                => `(trm_val val_gt [lang| $t1] [lang| $t2])
+  | `([lang| $t1 <= $t2])               => `(trm_val val_le [lang| $t1] [lang| $t2])
+  | `([lang| $t1 >= $t2])               => `(trm_val val_ge [lang| $t1] [lang| $t2])
+  | `([lang| -$t])                      => `(trm_val val_opp [lang| $t])
+  | `([lang| $t1 = $t2])                => `(trm_val val_eq [lang| $t1] [lang| $t2])
+  | `([lang| $t1 != $t2])               => `(trm_val val_neq [lang| $t1] [lang| $t2])
+  | `([lang| $t1 mod $t2])              => `(trm_val val_mod [lang| $t1] [lang| $t2])
+  | `([lang| ($t)]) => `([lang| $t])
+
+
+@[app_unexpander trm_val] def unexpandVal : Lean.PrettyPrinter.Unexpander
+  | `($(_) $x) =>
+    match x with
+    | `(val_unit) => `([lang| ()])
+    | `(val_int $n:num) => `([lang| $n:num])
+    | `(val_prim val_ref) => `([lang| ref])
+    | `(val_prim val_free) => `([lang| free])
+    | `(val_prim val_not) => `([lang| not])
+    | t => return t
+  | t => return t
+
+@[app_unexpander trm_app] def unexpandApp : Lean.PrettyPrinter.Unexpander := fun x =>
+  match x with
+  | `($(_) $op [lang| $t2]) =>
+    match op with
+    | `(trm_app $prim [lang| $t1]) =>
+      match prim with
+      | `(val_prim val_add) => `([lang| $t1 + $t2])
+      | `(val_prim val_mul) => `([lang| $t1 * $t2])
+      | `(val_prim val_sub) => `([lang| $t1 - $t2])
+      | `(val_prim val_div) => `([lang| $t1 / $t2])
+      | `(val_prim val_lt) => `([lang| $t1 < $t2])
+      | `(val_prim val_gt) => `([lang| $t1 > $t2])
+      | `(val_prim val_le) => `([lang| $t1 <= $t2])
+      | `(val_prim val_ge) => `([lang| $t1 >= $t2])
+      | `(val_prim val_eq) => `([lang| $t1 = $t2])
+      | `(val_prim val_neq) => `([lang| $t1 != $t2])
+      | `(val_prim val_mod) => `([lang| $t1 mod $t2])
+      | `(val_prim val_set) => `([lang| $t1 := $t2])
+      | _ => return x
+    | `(val_prim val_get) => `([lang| !$t2])
+    | `(val_prim val_neg) => `([lang| -$t2])
+    -- | `([lang| $f]) => `([lang| $f $t2])
+    | _ => return x
+  -- | `($(_) [lang| $t1] [lang| $t2]) => `([lang| $t1 $t2])
+  | t => return t
+
+@[app_unexpander trm_var] def unexpandVar : Lean.PrettyPrinter.Unexpander
+  | `($(_) $x:str) =>
+    let str := x.getString
+    let name := Lean.mkIdent $ Lean.Name.mkSimple str
+    `([lang| $name:ident])
+  | t => return t
+
+@[app_unexpander trm_seq] def unexpandSeq : Lean.PrettyPrinter.Unexpander
+  | `($(_) [lang| $t1] [lang| $t2]) => `([lang| $t1 ; $t2])
+  | t => return t
+
+@[app_unexpander trm_let] def unexpandLet : Lean.PrettyPrinter.Unexpander
+  | `($(_) $x:str [lang| $t1] [lang| $t2]) =>
+    let str := x.getString
+    let name := Lean.mkIdent $ Lean.Name.mkSimple str
+    `([lang| let $name := $t1 in $t2])
+  | t => return t
+
+@[app_unexpander trm_if] def unexpandIf : Lean.PrettyPrinter.Unexpander
+  | `($(_) [lang| $t1] [lang| $t2] [lang| $t3]) => `([lang| if $t1 then $t2 else $t3])
+  | t => return t
+
+@[app_unexpander trm_fun] def unexpandTFun : Lean.PrettyPrinter.Unexpander
+  | `($(_) $x:str [lang| fun $xs* => $t]) =>
+    let str := x.getString
+    let name := Lean.mkIdent $ Lean.Name.mkSimple str
+    `([lang| fun $name $xs* => $t])
+  | `($(_) $x:str [lang| $t]) =>
+    let str := x.getString
+    let name := Lean.mkIdent $ Lean.Name.mkSimple str
+    `([lang| fun $name => $t])
+  | t => return t
+
+@[app_unexpander val_fun] def unexpandVFun : Lean.PrettyPrinter.Unexpander
+  | `($(_) $x:str [lang| fun $xs* => $t]) =>
+    let str := x.getString
+    let name := Lean.mkIdent $ Lean.Name.mkSimple str
+    `([lang| fun $name $xs* => $t])
+  | `($(_) $x:str [lang| $t]) =>
+    let str := x.getString
+    let name := Lean.mkIdent $ Lean.Name.mkSimple str
+    `([lang| fun $name => $t])
+  | t => return t
+
+@[app_unexpander trm_fix] def unexpandTFix : Lean.PrettyPrinter.Unexpander
+  | `($(_) $f:str $x:str [lang| fun $xs* => $t]) =>
+    let f := f.getString
+    let x := x.getString
+    let nameF := Lean.mkIdent $ Lean.Name.mkSimple f
+    let nameX := Lean.mkIdent $ Lean.Name.mkSimple x
+    `([lang| fix $nameF $nameX $xs* => $t])
+  | `($(_) $f:str $x:str [lang| $t]) =>
+    let f := f.getString
+    let x := x.getString
+    let nameF := Lean.mkIdent $ Lean.Name.mkSimple f
+    let nameX := Lean.mkIdent $ Lean.Name.mkSimple x
+    `([lang| fix $nameF $nameX => $t])
+  | t => return t
+
+@[app_unexpander val_fix] def unexpandVFix : Lean.PrettyPrinter.Unexpander
+  | `($(_) $f:str $x:str [lang| fun $xs* => $t]) =>
+    let f := f.getString
+    let x := x.getString
+    let nameF := Lean.mkIdent $ Lean.Name.mkSimple f
+    let nameX := Lean.mkIdent $ Lean.Name.mkSimple x
+    `([lang| fix $nameF $nameX $xs* => $t])
+  | `($(_) $f:str $x:str [lang| $t]) =>
+    let f := f.getString
+    let x := x.getString
+    let nameF := Lean.mkIdent $ Lean.Name.mkSimple f
+    let nameX := Lean.mkIdent $ Lean.Name.mkSimple x
+    `([lang| fix $nameF $nameX => $t])
+  | t => return t
+
+@[app_unexpander trm_apps] def unexpandApps : Lean.PrettyPrinter.Unexpander
+  | `($(_) [lang| $f] [ $[[lang|$xs]],* ]) => `([lang| $f ( $xs,* )])
+  | t => return t
+
+@[app_unexpander trm_funs] def unexpandTFuns : Lean.PrettyPrinter.Unexpander
+  | `($(_) [ $xs:str,* ] [lang| $f]) =>
+    let xs := xs.getElems.map (Lean.mkIdent $ Lean.Name.mkSimple ·.getString)
+    `([lang| fun $xs* => $f])
+  | t => return t
+
+@[app_unexpander val_funs] def unexpandVFuns : Lean.PrettyPrinter.Unexpander
+  | `($(_) [ $xs:str,* ] [lang| $f]) =>
+    let xs := xs.getElems.map (Lean.mkIdent $ Lean.Name.mkSimple ·.getString)
+    `([lang| fun $xs* => $f])
+  | t => return t
+
+@[app_unexpander trm_fixs] def unexpandTFixs : Lean.PrettyPrinter.Unexpander
+  | `($(_) $f:str [ $xs:str,* ] [lang| $t]) =>
+    let xs := xs.getElems.map (Lean.mkIdent $ Lean.Name.mkSimple ·.getString)
+    let f := Lean.mkIdent $ Lean.Name.mkSimple f.getString
+    `([lang| fix $f $xs* => $t])
+  | t => return t
+
+@[app_unexpander val_fixs] def unexpandVFixs : Lean.PrettyPrinter.Unexpander
+  | `($(_) $f:str [ $xs:str,* ] [lang| $t]) =>
+    let xs := xs.getElems.map (Lean.mkIdent $ Lean.Name.mkSimple ·.getString)
+    let f := Lean.mkIdent $ Lean.Name.mkSimple f.getString
+    `([lang| fix $f $xs* => $t])
+  | t => return t
+
+
+-- #check [lang|
+--   fix f y z =>
+--     if f(y, z)
+--     then
+--       let y := 1 + 1 + () in
+--       let y := 1 + 1 in
+--       let z := ref(1) in
+--       y + z
+--     else
+--       let y := 1 + 1 in
+--       let z := 1 in
+--       y + z]
